progress

coq/confluence.v
@@ -9,6 +9,14 @@ Unset Strict Implicit.
 Unset Printing Implicit Defensive.
 Set Bullet Behavior "Strict Subproofs". 
 
+Lemma set2_Sub (T : finType) (p : pred T) (x y : T) (Hx : p x) (Hy : p y) :
+  [set Sub x Hx ; Sub y Hy] = [set z | val z \in [set x;y]] :> {set sig p}.
+Proof. apply/setP=>k. rewrite !inE -!val_eqE. done. Qed.
+
+Notation "'Σ' x .. y , p" :=
+  (sigT (fun x => .. (sigT (fun y => p%type)) ..))
+  (at level 200, x binder, y binder, right associativity).
+
 Notation IO := [set input; output].
 
 Section multigraph_plus.
@@ -18,7 +26,9 @@ Implicit Types (x y : G).
 Definition incident x e := x \in [set source e; target e].
 Definition edges_at x := [set e | incident x e].
 
-Lemma consistentD V : consistent (~: V) (~: \bigcup_(x in V) edges_at x).
+Definition edges_in (V : {set G}) := \bigcup_(x in V) edges_at x.
+
+Lemma consistentD V : consistent (~: V) (~: edges_in V).
 Admitted.
 
 Lemma consistentD1 x : consistent [set~ x] (~: edges_at x).
@@ -48,10 +58,16 @@ Variable (G : lgraph).
 
 
 Lemma arcC (e : edge G) x y u : 
-  arc e x u y <-> arc e y u x.
+  arc e x u y <-> arc e y u° x.
+Proof. 
+  rewrite /arc; split; move => [[-> -> A]|[-> -> A]].
 Admitted.
 
 Lemma add_edge_arc x y u : @arc (add_edge G x y u) None x u y.
+Admitted.
+
+Lemma add_edge_arc' x y x' y' u u' e : 
+  @arc G e x u y -> @arc (add_edge G x' u' y') (Some e) x u y.
 Admitted.
 
 Lemma edges_at_add_edgeT x u y z: z \in [set x;y] -> 
@@ -61,6 +77,9 @@ Admitted.
 Lemma edges_at_add_edgeN x u y z: z \notin [set x;y] -> 
   edges_at (add_edge G x y u) z = Some @: edges_at z.
 Admitted.
+
+Lemma edges_in1 (x : G) : edges_in [set x] = edges_at x. 
+Proof. by rewrite /edges_in big_set1. Qed.
 
 End lgraph_plus.
 
@@ -84,26 +103,34 @@ End DelVertices.
 Arguments del_vertices [G] V _.
 
 Section DelVertex.
-Variables (G : lgraph) (x : G) (Hx : x \notin IO).
+Variables (G : lgraph) (z : G) (Hz : z \notin IO).
 
-Lemma del_vertex_proof : [disjoint [set x] & IO].
+Lemma del_vertex_proof : [disjoint [set z] & IO].
 Admitted.
 
-Definition del_vertex := del_vertices [set x] del_vertex_proof.
+Definition del_vertex := del_vertices [set z] del_vertex_proof.
 
-Lemma edges_at_del_vertices z : 
-  edges_at del_vertex z = [set e | val e \notin edges_at x].
+
+Lemma edges_at_del_vertices (x : del_vertex) :
+  edges_at del_vertex x = [set e : edge del_vertex | val e \in edges_at (val x)].
 Admitted.
 
-Lemma edges_at_del_vertices0 z : edges_at (val z) \subset edges_at x ->
-  edges_at del_vertex z = set0.
+Lemma edges_at_del_vertices0 x : edges_at (val x) \subset edges_at z ->
+  edges_at del_vertex x = set0.
 Proof. rewrite edges_at_del_vertices. 
+Admitted.
+
+Lemma del_vertex_IO x (Hx : x \in [set~ z]) : x \notin IO -> (Sub x Hx : del_vertex) \notin IO.
+Proof. by rewrite !inE -!val_eqE /=. Qed.
+
+Lemma del_vertex_arc x y u e (Hx : x \in [set~ z]) (Hy : y \in [set~ z]) (He : e \in ~: edges_in [set z] ):
+  arc e x u y -> @arc del_vertex (Sub e He) (Sub x Hx) u (Sub y Hy). 
 Admitted.
 
 End DelVertex.
 
+Arguments arc : clear implicits.
 Arguments del_vertex : clear implicits.
-
 
 Definition del_edges (G : lgraph) (E : {set edge G}) := 
   point (remove_edges E) input output.
@@ -112,23 +139,36 @@ Arguments del_edges : clear implicits.
 Notation del_edge G e := (del_edges G [set e]).
 
 
+
+Lemma add_test_arc (G : lgraph) (e : edge G) x y z u a :
+  arc G e x u y -> arc (add_test G z a) e x u y.
+Admitted.
+
+Lemma edges_at_test (G : lgraph) a (x y : G) :
+  @edges_at _ _ (add_test G x a) y = edges_at y.
+Admitted.
+
+Arguments add_test_arc [G e x y z u a].
+
 Universe S.
 
 Variant Rule := RULE_V1 | RULE_V2 | RULE_E1 | RULE_E2.
 
 (* TOTHINK: Put the the add_test below the del_vertex to avoid the dependency? *)
 Inductive step : lgraph -> lgraph -> Type@{S} := 
-| step_v1 G x z e (Hz : z \notin IO) (Hx : x \in [set~ z]) u:  
-    arc e x u z -> edges_at z = [set e] ->
-    step G (add_test (del_vertex G z Hz) (Sub x Hx) [dom(u·vlabel z)])
+| step_v1 G x z e (Hz : z \notin IO) (Hx : (* x \in [set~ z]) *) x != z) u:  
+    arc G e x u z -> edges_at z = [set e] ->
+    step G (del_vertex (add_test G x [dom(u·vlabel z)]) z Hz)
+    (* step G (add_test (del_vertex G z Hz) (Sub x Hx) [dom(u·vlabel z)]) *)
 | step_v2 G x y z e1 e2 (Hz : z \notin IO) (Hx : x \in [set~ z]) (Hy : y \in [set~ z]) u v : 
-    arc e1 x u z -> arc e2 z v y -> edges_at z = [set e1;e2] -> e1 != e2 ->
+    arc G e1 x u z -> arc G e2 z v y -> edges_at z = [set e1;e2] -> e1 != e2 ->
+    (* step G (del_vertex (add_edge G x y (u·vlabel z·v)) z Hz). *)
     step G (add_edge (del_vertex G z Hz) (Sub x Hx) (Sub y Hy) (u·vlabel z·v))
 | step_e1 G e x : 
     source e = x -> target e = x -> 
     step G (add_test (del_edge G e) x [1∥elabel e])
 | step_e2 G e1 e2 x y u v : 
-    arc e1 x u y -> arc e2 x v y -> x != y ->
+    arc G e1 x u y -> arc G e2 x v y -> x != y ->
     step G (add_edge (del_edges G [set e1;e2]) x y (u∥v))
 .
 
@@ -151,16 +191,47 @@ Inductive steps: lgraph -> lgraph -> Type@{S} :=
   | trans_steps : CRelationClasses.Transitive steps.
 
 
-Notation "'Σ' x .. y , p" :=
-  (sigT (fun x => .. (sigT (fun y => p%type)) ..))
-  (at level 200, x binder, y binder, right associativity).
-
 Ltac GlGr :=
   match goal with 
     |- context[(steps ?G _ * steps ?H _)%type] => set Gl := G; set Gr := H
   end.
 
 Require Import set_tac.
+
+(* Ltac confluence_tac := *)
+
+(* Set Printing Existential Instances. *)
+
+Tactic Notation "inst" := 
+  unshelve instantiate (1 := ltac: (apply: id)); first try assumption.
+Tactic Notation "inst" tactic(tac) := 
+  try (unshelve instantiate (1 := ltac: (apply: id)); first abstract by tac).
+
+Notation "G  \  [ x , Hx ]" := (del_vertex G x Hx) (at level 30).
+
+(** liso lemmas *)
+
+Lemma cnvtst (u : test) : u° ≡ u.
+Admitted.
+
+Section liso.
+  Variable (G : lgraph).
+  
+  Lemma liso_del_tst x Hx y Hy a :
+    liso (add_test (G \ [x,Hx]) (Sub y Hy) a) (add_test G y a \ [x,Hx]).
+  Admitted.
+
+  Lemma liso_add_edgeC x y u : liso (add_edge G x y u) (add_edge G y x u°).
+  Admitted.
+
+  Lemma liso_add_edge_weq x y u v : u ≡ v -> liso (add_edge G x y u) (add_edge G x y v).
+  Admitted.
+End liso.
+
+Arguments edges_at [Lv Le] G _.
+Arguments edges_in [Lv Le] G _.
+
+Local Notation "⌈ x ⌉" := (Sub x _) (format "⌈ x ⌉") : sub_scope.
 
 Lemma local_confluence (G Gl Gr: lgraph) : 
   step G Gl -> step G Gr -> Σ Hl Hr, steps Gl Hl * steps Gr Hr * liso Hl Hr.
@@ -172,18 +243,71 @@ Proof.
     - case: (W _ _ _ _ SS) => Hr [Hl] [[Sr Sl] l]. 
       exists Hl; exists Hr. split => //. exact: liso_sym. }
   destruct S as [G x z e Hz Hx u Ae Iz|*|*|*]; 
-  destruct S' as [*|G' x' y' z' e1' e2' Hz' Hx' Hy' u' v' Ae1' Ae2' Iz' D|*|*]; try done; move => _; GlGr.
+  destruct S' as [*|G x' y' z' e1' e2' Hz' Hx' Hy' u' v' Ae1' Ae2' Iz' D'|*|*]; try done; move => _.
   - (* Case V1 / V1 *) admit.
   - (* Case V1 / V2 *) 
-    case: (altP (z =P y')) => [?|xDy'].
-    + subst y'. 
+    have Dz : z != z' by admit. (* different degree *)
+    case: (boolP (z \in [set x';y'])) => [z_xy'|xD'].
+    + wlog ? : x' y' Hx' Hy' e1' e2' u' v' Ae1' Ae2' Iz' D' {z_xy'} / z = y'. 
+      { move => W. rewrite !inE in z_xy'. case/orb_sum : z_xy' => /eqP ?; subst z.
+        - move/(_ _ _ Hy' Hx' e2' e1' v'° u'°) in W. 
+          case: W; rewrite -?arcC // 1?setUC 1?eq_sym //. 
+          move => Hl [Hr] [[steps_l steps_r] liso_lr].
+          exists Hl; exists Hr. repeat split => //. apply: trans_steps steps_r. 
+          apply: liso_step. rewrite -> liso_add_edgeC. apply: liso_add_edge_weq. 
+          by rewrite !cnvdot cnvtst dotA.
+        - exact: W Iz' _ _ . }
+      subst z. 
       have [? ?] : e2' = e /\ z' = x ; subst. admit. 
       do 2 eexists; repeat split. 
-      * apply step_step. (* x is preserved and its only incident edge in Gl is  e1' *)
-      * apply step_step. apply step_v1 with None. apply add_edge_arc. 
+      * (* x is preserved and its only incident edge in Gl is  e1' *)
+        apply step_step. apply: step_v1. 
+        3: apply: del_vertex_arc. 6:apply: add_test_arc Ae1'.
+        inst (move: (Hy'); rewrite !inE eq_sym).
+        exact: del_vertex_IO.
+        by rewrite -val_eqE /= -in_set1 -in_setC. 
+        admit. 
+        admit.
+        rewrite edges_at_del_vertices edges_at_test /= Iz'. admit. 
+      * (* the x'z-edge is now the only edge incident at z *)
+        apply step_step. apply step_v1 with None. 2:apply add_edge_arc. admit.
         rewrite edges_at_add_edgeT ?inD //. 
-        rewrite edges_at_del_vertices0 ?imset0 ?setU0 //= Iz Iz'. admit.
-      * admit.
+        rewrite edges_at_del_vertices0 ?imset0 ?setU0 //= Iz Iz'. apply: subsetUr. 
+      * inst (exact: del_vertex_IO). 
+        (* repeat match goal with |- context [Sub _ (?x ?y)] => let S := fresh "sub" in set S := x y end. *)
+        (* set X := _ _ _ _ _ _ _ _ _ _. *)
+        (* erewrite -> liso_del_tst. *) admit.
+    + (* the independent case *)
+      have He1 : e1' \in ~: edges_in (G[tst x <- [dom (u·vlabel z)]]) [set z]. admit.
+      have He2 : e2' \in ~: edges_in (G[tst x <- [dom (u·vlabel z)]]) [set z]. admit.
+      have He : e \in ~: edges_in G [set z']. admit.
+      have D : x != z'. admit. (* both edges at z' lead to vertices distinct from z *)
+      do 2 eexists; repeat split.
+      * apply step_step. apply: step_v2. 
+        4,5: apply: del_vertex_arc; last apply: add_test_arc.
+        7: apply Ae1'. 9: apply Ae2'.
+        (* side conditions - should be automatable *)
+        inst (rewrite !inE eq_sym).  
+        exact: del_vertex_IO.
+        inst set_tac.
+        abstract (rewrite !inE -val_eqE /=; set_tac).
+        inst set_tac. 
+        abstract (rewrite !inE -val_eqE /=; by set_tac). 
+        done.
+        done.
+        abstract (by rewrite edges_at_del_vertices edges_at_test /= Iz' set2_Sub).
+        by rewrite -val_eqE. 
+      * apply: step_step. apply: step_v1. 
+        3: apply: add_edge_arc'; last apply: del_vertex_arc; last apply Ae.
+        inst set_tac.
+        exact: del_vertex_IO.
+        inst set_tac. 
+        by rewrite -val_eqE. 
+        done.
+        admit.
+      * Open Scope sub_scope.
+        set X := del_vertex_IO _ _ _. set X' := del_vertex_IO _ _ _.
+        
   - (* Case V1 / E1 *) admit.
   - (* Case V1 / E2 *) admit.
   - (* Case V2 / V2 *) admit.
